10/28 pre-meeting update

src/del/semantics/consistencyDEL.lean
@@ -1,19 +1,21 @@
 -- Following the textbook "Dynamic Epistemic Logic" by 
 -- Hans van Ditmarsch, Wiebe van der Hoek, and Barteld Kooi
 
-import basicmodal.language basicmodal.syntax.syntax 
-import basicmodal.semantics.semantics basicmodal.syntax.syntaxlemmas
-import basicmodal.syntax.soundness order.zorn data.set.basic
+import del.languageDEL del.syntax.syntaxDEL 
+import del.semantics.semanticsDEL del.syntax.syntaxlemmasDEL
+import del.syntax.soundnessDEL order.zorn data.set.basic
 local attribute [instance] classical.prop_decidable
 
-open prfK
+open prfPA
+variables {agents : Type}
+
 
 ---------------------- Consistency ----------------------
 
-def sem_cons (AX : ctx) := ¬ global_sem_csq AX ⊥ 
+def sem_cons (AX : ctx agents) := ¬ global_sem_csq AX ⊥ 
 attribute [class] sem_cons
 
-lemma sem_consK : sem_cons ∅ :=
+lemma sem_consPA : sem_cons ∅ :=
 begin
 rw sem_cons,
 rw global_sem_csq, 
@@ -29,126 +31,126 @@ exact false.elim h1, rw forces,
 trivial 
 end
 
-lemma sem_consT : sem_cons T_axioms :=
-begin
-rw sem_cons, rw global_sem_csq,
-push_neg,
-let f : frame := 
-{ states := ℕ,
-  h := ⟨0⟩,
-  rel := λ x y, x = y},
-use f, let v := λ n x, true,
-use v, let x := 42, use x,
-split, intros φ y h1, 
-cases h1 with ψ h1, subst h1,
-intro h1, apply h1 y,
-exact rfl,
-rw forces, trivial
-end
+-- lemma sem_consT : sem_cons T_axioms :=
+-- begin
+-- rw sem_cons, rw global_sem_csq,
+-- push_neg,
+-- let f : frame := 
+-- { states := ℕ,
+--   h := ⟨0⟩,
+--   rel := λ x y, x = y},
+-- use f, let v := λ n x, true,
+-- use v, let x := 42, use x,
+-- split, intros φ y h1, 
+-- cases h1 with ψ h1, subst h1,
+-- intro h1, apply h1 y,
+-- exact rfl,
+-- rw forces, trivial
+-- end
 
-lemma sem_consS4 : sem_cons S4_axioms :=
-begin
-rw sem_cons, rw global_sem_csq, push_neg,
-let f : frame := 
-{ states := ℕ,
-  h := ⟨0⟩,
-  rel := λ x y, x = y},
-use f, let v := λ n x, true,
-use v, let x := 42, use x,
-split, 
-intros φ y h1,
-rw S4_axioms at h1, cases h1,
-cases h1 with ψ h1, subst h1,
-intro h1, apply h1 y,
-exact rfl,
-cases h1 with ψ h1, subst h1,
-intro h1, rw forces at *,
-simp at *, rw forces, 
-simp at *, exact h1,
-rw forces, trivial
-end
+-- lemma sem_consS4 : sem_cons S4_axioms :=
+-- begin
+-- rw sem_cons, rw global_sem_csq, push_neg,
+-- let f : frame := 
+-- { states := ℕ,
+--   h := ⟨0⟩,
+--   rel := λ x y, x = y},
+-- use f, let v := λ n x, true,
+-- use v, let x := 42, use x,
+-- split, 
+-- intros φ y h1,
+-- rw S4_axioms at h1, cases h1,
+-- cases h1 with ψ h1, subst h1,
+-- intro h1, apply h1 y,
+-- exact rfl,
+-- cases h1 with ψ h1, subst h1,
+-- intro h1, rw forces at *,
+-- simp at *, rw forces, 
+-- simp at *, exact h1,
+-- rw forces, trivial
+-- end
 
-lemma sem_consS5 : sem_cons S5_axioms :=
-begin
-rw sem_cons, rw global_sem_csq, push_neg,
-let f : frame := 
-{ states := ℕ,
-  h := ⟨0⟩,
-  rel := λ x y, x = y},
-use f, let v := λ n x, true,
-use v, let x := 42, use x,
-split, 
-intros φ y h1,
-rw S5_axioms at h1, cases h1,
-cases h1 with ψ h1, subst h1,
-intro h1, apply h1 y,
-exact rfl,
-cases h1 with ψ h1, subst h1,
-intro h1, rw forces at *,
-simp at *, rw forces, 
-exact h1,
-rw forces, trivial
-end
+-- lemma sem_consS5 : sem_cons S5_axioms :=
+-- begin
+-- rw sem_cons, rw global_sem_csq, push_neg,
+-- let f : frame := 
+-- { states := ℕ,
+--   h := ⟨0⟩,
+--   rel := λ x y, x = y},
+-- use f, let v := λ n x, true,
+-- use v, let x := 42, use x,
+-- split, 
+-- intros φ y h1,
+-- rw S5_axioms at h1, cases h1,
+-- cases h1 with ψ h1, subst h1,
+-- intro h1, apply h1 y,
+-- exact rfl,
+-- cases h1 with ψ h1, subst h1,
+-- intro h1, rw forces at *,
+-- simp at *, rw forces, 
+-- exact h1,
+-- rw forces, trivial
+-- end
 
 
 -- Any axiom system that is consistent does not prove false
-lemma nprfalse (AX : ctx) (hax : sem_cons AX) : ¬ prfK AX ⊥ :=
+lemma nprfalse (AX : ctx agents) (hax : sem_cons AX) : ¬ prfPA AX ⊥ :=
 begin
-have h1 : ¬ global_sem_csq AX ⊥ → ¬ prfK AX ⊥, 
-{have h2 : prfK AX ⊥ → global_sem_csq AX ⊥, from soundness AX ⊥, 
+have h1 : ¬ global_sem_csq AX ⊥ → ¬ prfPA AX ⊥, 
+{have h2 : prfPA AX ⊥ → global_sem_csq AX ⊥, from soundnessPA AX ⊥, 
 rw ←not_imp_not at h2, exact h2},
 apply h1, exact hax
 end
 
-lemma prnot_to_notpr (φ : form) (AX : ctx) (hax : sem_cons AX) : 
-  prfK AX (¬φ) → ¬ prfK AX φ :=
+lemma prnot_to_notpr (φ : formPA agents) (AX : ctx agents) (hax : sem_cons AX) : 
+  prfPA AX (~φ) → ¬ prfPA AX φ :=
 begin
-intro h1, by_contradiction h2, simp at *,
-have h3 : prfK AX ⊥, from mp (mp pl5 contra_equiv_false) (mp (mp pl4 h2) h1),
-have h4 : ¬ prfK AX ⊥, from nprfalse AX hax,
+intro h1, by_contradiction h2,
+have h3 : prfPA AX ⊥, from mp (mp pl5 contra_equiv_false) (mp (mp pl4 h2) h1),
+have h4 : ¬ prfPA AX ⊥, from nprfalse AX hax,
 exact absurd h3 h4
 end 
 
-lemma pr_to_notprnot (φ : form) (AX : ctx) (hax : sem_cons AX) : 
-  prfK AX φ → ¬ prfK AX (¬φ) :=
+lemma pr_to_notprnot (φ : formPA agents) (AX : ctx agents) (hax : sem_cons AX) : 
+  prfPA AX φ → ¬ prfPA AX (~φ) :=
 begin
-have h1 : prfK AX (¬φ) → ¬ prfK AX φ, from prnot_to_notpr φ AX hax,
+have h1 : prfPA AX (~φ) → ¬ prfPA AX φ, from prnot_to_notpr φ AX hax,
 rw ←not_imp_not at h1, intro h2, apply h1, rw not_not, exact h2,
 end 
 
 -- finite conjunction of formulas
-def fin_conj : list form → form
-  | []  := ⊤
+def fin_conj : list (formPA agents) → formPA agents
+  | []  := ~formPA.bot
   | (φ::φs) := φ & (fin_conj φs)
 
 -- a few helper lemmas about finite conjunctions
-lemma fin_conj_simp {Γ : ctx} : ∀ ψ : form, prfK Γ (¬fin_conj [ψ, ¬ψ]) :=
+lemma fin_conj_simp {Γ : ctx agents} : ∀ ψ : formPA agents, prfPA Γ (~fin_conj [ψ, ~ψ]) :=
 begin
-intro ψ, simp, rw fin_conj, rw fin_conj, rw fin_conj, simp,
-have h2 : (prfK Γ (((¬ψ)&⊤) ↔ (¬ψ)) → 
-  (prfK Γ (¬(ψ & ((¬ψ)&⊤))) ↔ prfK Γ (¬(ψ & (¬ψ))))), 
+intro ψ, rw fin_conj, rw fin_conj, rw fin_conj,
+have h2 : (prfPA Γ (((~ψ)&(~⊥)) ↔ (~ψ)) → 
+  (prfPA Γ (~(ψ & ((~ψ)&(~⊥)))) ↔ prfPA Γ (~(ψ & (~ψ))))), 
   from not_and_subst,
 simp at h2,
 specialize h2 phi_and_true, cases h2,
 exact h2_mpr not_contra
 end
 
-lemma imp_conj_imp_imp {Γ : ctx} {φ ψ χ : form} {L : list form} : 
-  prfK Γ ((fin_conj (φ::L)) ⊃ ψ) ↔ prfK Γ (fin_conj L ⊃ (φ ⊃ ψ)) :=
+lemma imp_conj_imp_imp {Γ : ctx agents} {φ ψ χ : formPA agents} {L : list (formPA agents)} : 
+  prfPA Γ ((fin_conj (φ::L)) ⊃ ψ) ↔ prfPA Γ (fin_conj L ⊃ (φ ⊃ ψ)) :=
 begin
 split, 
 intro h, dsimp [fin_conj] at h, rw and_right_imp at h, exact h,
 intro h, dsimp [fin_conj], rw and_right_imp, exact h
 end
 
-lemma fin_conj_cons_imp {Γ : ctx} {φ b : form} {L : list form} : 
- prfK Γ (fin_conj (φ::L) ⊃ (φ ⊃ b)) → prfK Γ (fin_conj L ⊃ (φ ⊃ b)) :=
+lemma fin_conj_cons_imp {Γ : ctx agents} {φ b : formPA agents} {L : list (formPA agents)} : 
+ prfPA Γ (fin_conj (φ::L) ⊃ (φ ⊃ b)) → prfPA Γ (fin_conj L ⊃ (φ ⊃ b)) :=
 begin
 intro h, rw imp_conj_imp_imp at h, rw imp_imp_iff_imp at h, exact h, exact φ,
 end
 
-lemma fin_conj_append {Γ : ctx} {L L' : list form} :
-  prfK Γ ((fin_conj L' & fin_conj L) ↔ (fin_conj (L' ++ L))) :=
+lemma fin_conj_append {Γ : ctx agents} {L L' : list (formPA agents)} :
+  prfPA Γ ((fin_conj L' & fin_conj L) ↔ (fin_conj (L' ++ L))) :=
 begin
 induction L', rw fin_conj,
 exact (mp (mp pl4 (cut (mp pl6 and_switch) (mp pl5 phi_and_true))) 
@@ -157,19 +159,19 @@ exact mp (mp pl4 (cut (mp pl5 and_commute) (imp_and_imp (mp pl5 L'_ih))))
   (cut iden (cut (imp_and_imp (mp pl6 L'_ih)) (mp pl6 and_commute)))
 end 
 
-lemma fin_conj_empty {AX : ctx} {L : list form} (hax : sem_cons AX) :
-  L = [] → ¬ prfK AX (fin_conj L ⊃ ⊥) :=
+lemma fin_conj_empty {AX : ctx agents} {L : list (formPA agents)} (hax : sem_cons AX) :
+  L = [] → ¬ prfPA AX (fin_conj L ⊃ ⊥) :=
 begin
-intro h1, subst h1, rw fin_conj, simp at *,
-have h1 : prfK AX (¬⊥), from iden,
-simp at *, by_contradiction h2,
-have h3 : prfK AX ⊥, from mp h2 h1,
-have h4 : ¬ prfK AX ⊥, from nprfalse AX hax,
+intro h1, subst h1, rw fin_conj,
+have h1 : prfPA AX (~⊥), from iden,
+by_contradiction h2,
+have h3 : prfPA AX ⊥, from mp h2 h1,
+have h4 : ¬ prfPA AX ⊥, from nprfalse AX hax,
 exact absurd h3 h4
 end 
 
-lemma fin_conj_repeat_helper {AX : ctx} {θ : form} {L : list form} (hax : sem_cons AX) :
-  (∀ ψ ∈ L, ψ = θ) → prfK AX (θ ⊃ fin_conj L) :=
+lemma fin_conj_repeat_helper {AX : ctx agents} {θ : formPA agents} {L : list (formPA agents)} (hax : sem_cons AX) :
+  (∀ ψ ∈ L, ψ = θ) → prfPA AX (θ ⊃ fin_conj L) :=
 begin
 intros h1, induction L,
 exact mp pl1 iden,
@@ -179,8 +181,8 @@ specialize L_ih h2, subst h1,
 exact cut (mp double_imp pl4) (imp_and_and_imp (mp (mp pl4 iden) L_ih)),
 end
 
-lemma fin_conj_repeat {AX : ctx} {φ : form} {L : list form} (hax : sem_cons AX) :
-  (∀ ψ ∈ L, ψ = ¬φ) → prfK AX (¬fin_conj L) → prfK AX φ :=
+lemma fin_conj_repeat {AX : ctx agents} {φ : formPA agents} {L : list (formPA agents)} (hax : sem_cons AX) :
+  (∀ ψ ∈ L, ψ = ~φ) → prfPA AX (~fin_conj L) → prfPA AX φ :=
 begin
 intros h1 h2, induction L,
 rw fin_conj at h2,
@@ -189,19 +191,20 @@ have h4 := nprfalse AX hax,
 exact absurd h3 h4,
 repeat {rw fin_conj at *}, simp at *,
 cases h1 with h1 h3, 
-have h5 : prfK AX ((¬fin_conj L_tl) ⊃ ¬(¬φ)), from contrapos.mpr (fin_conj_repeat_helper hax h3),
+have h5 : prfPA AX ((¬fin_conj L_tl) ⊃ ¬(¬φ)), from contrapos.mpr (fin_conj_repeat_helper hax h3),
 subst h1,
 exact (mp (mp pl3 (contrapos.mpr (cut h5 dne))) 
   (contrapos.mpr (cut ((demorgans.mp) (mp (mp pl6 (iff_not and_switch)) h2)) dne)))
 end
 
-lemma fin_conj_box2 {AX : ctx} {φ ψ : form} : prfK AX ((□φ & □ψ) ⊃ □(φ & ψ)) :=
+lemma fin_conj_box2 {AX : ctx agents} {φ ψ : formPA agents} {a : agents} : 
+  prfPA AX (((K a φ) & K a ψ) ⊃ K a (φ & ψ)) :=
 begin
 exact (mp double_imp (cut2 pl6 (cut pl5 (cut (mp kdist (nec pl4)) kdist))))
 end
 
-lemma fin_conj_boxn {AX : ctx} {L : list form} : 
-  prfK AX ((fin_conj (list.map □ L)) ⊃ (□(fin_conj L))) :=
+lemma fin_conj_boxn {AX : ctx agents} {L : list (formPA agents)} {a : agents} : 
+  prfPA AX ((fin_conj (list.map (K a) L)) ⊃ (K a (fin_conj L))) :=
 begin
 induction L,
 rw fin_conj, simp at *, rw fin_conj,
@@ -213,7 +216,7 @@ exact (cut h1 fin_conj_box2)
 end
 
 
-lemma listempty {Γ : ctx} {L : list form} :
+lemma listempty {Γ : ctx agents} {L : list (formPA agents)} :
   (∀ φ ∈ L, φ ∈ Γ) → Γ = ∅ → L = [] := 
 begin
 intros h1 h2,
@@ -229,20 +232,20 @@ end
 
 
 -- consistency for a finite set of formulas L
-def fin_ax_consist (AX : ctx) (L : list form) := ¬ prfK AX (fin_conj L ⊃ ⊥)
+def fin_ax_consist (AX : ctx agents) (L : list (formPA agents)) := ¬ prfPA AX (fin_conj L ⊃ ⊥)
 
 
 -- consistency for an arbitrary set of formulas Γ
-def ax_consist (AX Γ : ctx) :=
-  ∀ L : list form, (∀ ψ ∈ L, ψ ∈ Γ) → fin_ax_consist AX L
+def ax_consist (AX Γ : ctx agents) :=
+  ∀ L : list (formPA agents), (∀ ψ ∈ L, ψ ∈ Γ) → fin_ax_consist AX L
 
 
 -- Γ is maximally ax-consistent
-def max_ax_consist (AX Γ : ctx) := 
+def max_ax_consist (AX Γ : ctx agents) := 
   ax_consist AX Γ ∧ (∀ Γ', Γ ⊂ Γ' → ¬ ax_consist AX Γ')
 
 
-lemma max_imp_ax {AX Γ : ctx} : max_ax_consist AX Γ → ax_consist AX Γ :=
+lemma max_imp_ax {AX Γ : ctx agents} : max_ax_consist AX Γ → ax_consist AX Γ :=
 begin
 intro h1, rw max_ax_consist at h1, cases h1, exact h1_left
 end
@@ -253,19 +256,19 @@ if everything in L is in Gamma or equal to phi, and you can prove conj L ⊃ b,
 then there is a list L', such that everything in L' is in Gamma, and you can 
 prove conj L' ⊃ (phi ⊃ b)
 -/
-lemma five_helper (AX : ctx) : 
-  ∀ Γ : ctx, ∀ φ : form, ∀ L : list form, ∀ b : form, 
-  (∀ ψ ∈ L, ψ ∈ Γ ∨ ψ = φ) → prfK AX (fin_conj L ⊃ b) → ∃ L',
-  (∀ ψ ∈ L', ψ ∈ Γ) ∧ prfK AX (fin_conj L' ⊃ (φ ⊃ b)) :=
+lemma five_helper (AX : ctx agents) : 
+  ∀ Γ : ctx agents, ∀ φ : formPA agents, ∀ L : list (formPA agents), ∀ b : formPA agents, 
+  (∀ ψ ∈ L, ψ ∈ Γ ∨ ψ = φ) → prfPA AX (fin_conj L ⊃ b) → ∃ L',
+  (∀ ψ ∈ L', ψ ∈ Γ) ∧ prfPA AX (fin_conj L' ⊃ (φ ⊃ b)) :=
 begin
 intros Γ φ L b h1 h2, 
 revert b, 
 induction L,
-{intros b h2, existsi ([] : list form), split, 
+{intros b h2, existsi ([] : list (formPA agents)), split, 
 intros ψ h3, exfalso, apply list.not_mem_nil ψ h3, 
 dsimp [fin_conj] at *, exact imp_if_imp_imp h2},
 {intros b h2,
-have h1a : ∀ (ψ : form), ψ ∈ L_tl → ψ ∈ Γ ∨ ψ = φ, 
+have h1a : ∀ (ψ : formPA agents), ψ ∈ L_tl → ψ ∈ Γ ∨ ψ = φ, 
   {intros ψ h2, specialize h1 ψ, 
   have h3 := list.subset_cons L_hd L_tl,
   have h4 := list.mem_cons_of_mem L_hd h2, 
@@ -274,50 +277,50 @@ specialize L_ih h1a,
 have h1b: L_hd ∈ Γ ∨ L_hd = φ, 
   {apply h1 L_hd, left, refl},
 cases h1b, 
-have h3 : prfK AX (fin_conj L_tl ⊃ (L_hd ⊃ b)), 
+have h3 : prfPA AX (fin_conj L_tl ⊃ (L_hd ⊃ b)), 
   from and_right_imp.mp h2,
 specialize L_ih (L_hd ⊃ b) h3,
-cases L_ih with L' ih, existsi (L_hd::L' : list form),
+cases L_ih with L' ih, existsi (L_hd::L' : list (formPA agents)),
 cases ih, split, intros ψ h4, cases h4, 
 subst h4, exact h1b, 
 apply ih_left ψ h4, rw imp_shift at ih_right,
 rw ←imp_conj_imp_imp at ih_right, exact ih_right,
-have h3 : prfK AX (fin_conj (L_hd::L_tl) ⊃ b), 
+have h3 : prfPA AX (fin_conj (L_hd::L_tl) ⊃ b), 
 exact h2, exact b,
 specialize L_ih (φ ⊃ b),
-have h5 : prfK AX (fin_conj (L_hd :: L_tl) ⊃ b) → 
-  prfK AX (fin_conj L_tl ⊃ (L_hd ⊃ b)), 
+have h5 : prfPA AX (fin_conj (L_hd :: L_tl) ⊃ b) → 
+  prfPA AX (fin_conj L_tl ⊃ (L_hd ⊃ b)), 
   from and_right_imp.mp,
 specialize h5 h2,
-have h6 : prfK AX (fin_conj L_tl ⊃ (φ ⊃ b)), 
+have h6 : prfPA AX (fin_conj L_tl ⊃ (φ ⊃ b)), 
   from eq.subst h1b h5,
 specialize L_ih h6, cases L_ih with L' ih, 
-cases ih, existsi (L' : list form), split, 
+cases ih, existsi (L' : list (formPA agents)), split, 
 exact ih_left, exact imp_imp_iff_imp.mp ih_right}
 end
 
 -- Lemma 5 from class notes
-lemma five (AX : ctx) : 
-  ∀ Γ : ctx, ∀ φ : form, ¬ ax_consist AX (Γ un φ) → ∃ L',
-  (∀ ψ ∈ L', ψ ∈ Γ) ∧ prfK AX (fin_conj L' ⊃ ¬φ) :=
+lemma five (AX : ctx agents) : 
+  ∀ Γ : ctx agents, ∀ φ : formPA agents, ¬ ax_consist AX (Γ un φ) → ∃ L',
+  (∀ ψ ∈ L', ψ ∈ Γ) ∧ prfPA AX (fin_conj L' ⊃ ~φ) :=
 begin
 intro Γ, intro φ, intro h1, simp at *, rw ax_consist at h1, 
 push_neg at h1,
 cases h1 with L h1,
-have h2 : (∀ ψ ∈ L, ψ ∈ Γ ∨ ψ = φ) → prfK AX (fin_conj L ⊃ ⊥) → ∃ L',
-  (∀ ψ ∈ L', ψ ∈ Γ) ∧ prfK AX (fin_conj L' ⊃ (φ ⊃ ⊥)), from five_helper AX Γ φ L ⊥,
+have h2 : (∀ ψ ∈ L, ψ ∈ Γ ∨ ψ = φ) → prfPA AX (fin_conj L ⊃ ⊥) → ∃ L',
+  (∀ ψ ∈ L', ψ ∈ Γ) ∧ prfPA AX (fin_conj L' ⊃ (φ ⊃ ⊥)), from five_helper AX Γ φ L ⊥,
 cases h1,
-have h3 : (∀ (ψ : form), ψ ∈ L → ψ ∈ Γ ∨ ψ = φ), 
+have h3 : (∀ (ψ : formPA agents), ψ ∈ L → ψ ∈ Γ ∨ ψ = φ), 
 {intros ψ this, specialize h1_left ψ this, exact or.swap h1_left},
 specialize h2 h3, apply h2, rw fin_ax_consist at h1_right, rw not_not at h1_right,
 exact h1_right,
 end
 
 
-lemma six_helper (AX Γ : ctx) (h : ax_consist AX Γ) :
-max_ax_consist AX Γ → ∀ φ : form, φ ∈ Γ ∨ (¬φ) ∈ Γ :=
+lemma six_helper (AX Γ : ctx agents) (h : ax_consist AX Γ) :
+max_ax_consist AX Γ → ∀ φ : formPA agents, φ ∈ Γ ∨ (~φ) ∈ Γ :=
 begin
-intros h1 φ, simp, rw or_iff_not_and_not, by_contradiction h2,
+intros h1 φ, rw or_iff_not_and_not, by_contradiction h2,
 cases h2 with h2l h2r, rw max_ax_consist at h1,
 cases h1 with h1l h1r, clear h, 
 have h2 := h1r (Γ un φ), have h3 := h1r (Γ un ¬φ),
@@ -328,14 +331,14 @@ have h5 : ¬ax_consist AX (Γ un φ),
 clear h2 h3, simp at *, have h6 := five AX Γ φ _, have h7 := five AX Γ (¬φ) _, 
 cases h6 with L' h6, cases h7 with L h7, dsimp at *, cases h6 with h6l h6r,
 cases h7 with h7l h7r,
-have h8 : prfK AX ((fin_conj L' & fin_conj L) ⊃ ((¬φ) & ¬¬φ)), 
+have h8 : prfPA AX ((fin_conj L' & fin_conj L) ⊃ ((¬φ) & ¬¬φ)), 
 from imp_and_and_imp (mp (mp pl4 h6r) h7r),
 simp at h8,
 rw ax_consist at h1l,
-have h12: prfK AX ((fin_conj (L' ++ L)) ⊃ ⊥), 
+have h12: prfPA AX ((fin_conj (L' ++ L)) ⊃ ⊥), 
 from cut (mp pl6 fin_conj_append) (cut h8 (mp pl5 contra_equiv_false)),
 specialize h1l (L' ++ L), rw fin_ax_consist at h1l,
-have h13: (∀ (ψ : form), ψ ∈ L' ++ L → ψ ∈ Γ), 
+have h13: (∀ (ψ : formPA agents), ψ ∈ L' ++ L → ψ ∈ Γ), 
 intro ψ, specialize h6l ψ, specialize h7l ψ, intro h13,
 rw list.mem_append at h13, cases h13, exact h6l h13, exact h7l h13,
 specialize h1l h13, exact absurd h12 h1l,
@@ -344,8 +347,8 @@ exact h5,
 end
 
 -- lemma 6 from class notes
-lemma six (AX Γ : ctx) (h : ax_consist AX Γ) :
-max_ax_consist AX Γ ↔ ∀ φ, (φ ∈ Γ ∨ (¬φ) ∈ Γ) ∧ ¬(φ ∈ Γ ∧ (¬φ) ∈ Γ) :=
+lemma six (AX Γ : ctx agents) (h : ax_consist AX Γ) :
+max_ax_consist AX Γ ↔ ∀ φ, (φ ∈ Γ ∨ (~φ) ∈ Γ) ∧ ¬(φ ∈ Γ ∧ (~φ) ∈ Γ) :=
 begin 
 simp, split, 
 intro h1, intro φ, 
@@ -353,11 +356,11 @@ split, exact six_helper AX Γ h h1 φ,
 {rw ←not_and, by_contradiction h2,
 cases h2 with h2 h3,
 rw ax_consist at h,
-specialize h ([φ, ¬φ]), simp at *,
-have h4 : (∀ (ψ : form), ψ = φ ∨ ψ = ¬φ → ψ ∈ Γ), 
-{intros ψ h4, simp at *, cases h4, subst h4, exact h2, subst h4, exact h3},
+specialize h ([φ, ~φ]), simp at *,
+have h4 : (∀ (ψ : formPA agents), ψ = φ ∨ ψ = ~φ → ψ ∈ Γ), 
+{intros ψ h4, cases h4, subst h4, exact h2, subst h4, exact h3},
 specialize h h4, rw fin_ax_consist at h, 
-have h5 : prfK AX (¬fin_conj [φ, ¬φ]), from fin_conj_simp φ, 
+have h5 : prfPA AX (~fin_conj [φ, ~φ]), from fin_conj_simp φ, 
 exact absurd h5 h},
 intro h1, rw max_ax_consist, split, exact h,
 intros Γ' h2,
@@ -368,21 +371,21 @@ apply (exists.elim h3_right), simp, intros ψ h4 h5,
 specialize h1 ψ, cases h1,
 cases h1_left,
 apply absurd h1_left h5,
-have h6 : (¬ψ) ∈ Γ', from set.mem_of_subset_of_mem h3_left h1_left,
+have h6 : (~ψ) ∈ Γ', from set.mem_of_subset_of_mem h3_left h1_left,
 rw ax_consist, 
 push_neg,
-existsi ([ψ,¬ψ] : list form),
+existsi ([ψ,~ψ] : list (formPA agents)),
 simp, split, intros φ h7, cases h7, subst h7, exact h4, 
 subst h7, exact h6, rw fin_ax_consist, rw not_not,
 exact fin_conj_simp ψ
 end
 
-lemma ex1help {AX Γ : ctx} {φ : form} {L L' : list form} :
-  (∀ ψ ∈ L, ψ ∈ Γ) → prfK AX (fin_conj L ⊃ φ) → (∀ ψ ∈ L', ψ ∈ (insert φ Γ)) 
-  → ∃ L'' : list form, (∀ ψ ∈ L'', ψ ∈ Γ) ∧ prfK AX (fin_conj L'' ⊃ fin_conj L') :=
+lemma ex1help {AX Γ : ctx agents} {φ : formPA agents} {L L' : list (formPA agents)} :
+  (∀ ψ ∈ L, ψ ∈ Γ) → prfPA AX (fin_conj L ⊃ φ) → (∀ ψ ∈ L', ψ ∈ (insert φ Γ)) 
+  → ∃ L'' : list (formPA agents), (∀ ψ ∈ L'', ψ ∈ Γ) ∧ prfPA AX (fin_conj L'' ⊃ fin_conj L') :=
 begin
 intros h1 h2 h3, induction L',
-existsi ([] : list form),
+existsi ([] : list (formPA agents)),
 split,
 intros ψ h4, exact false.elim h4,
 exact iden,
@@ -391,7 +394,7 @@ specialize L'_ih h4,
 cases L'_ih with L'' L'_ih,
 cases L'_ih with ih1 ih2,
 cases h3, 
-existsi (L''++L : list form),
+existsi (L''++L : list formPA agents),
 split,
 simp at *, intros ψ h2,
 cases h2 with h2 h5,
@@ -399,13 +402,13 @@ exact ih1 ψ h2,
 exact h1 ψ h5,
 subst h3, 
 exact (cut (mp pl6 fin_conj_append) (cut (mp pl5 and_switch) (imp_and_and_imp (mp (mp pl4 h2) ih2)))),
-existsi (L'_hd::L'' : list form),
+existsi (L'_hd::L'' : list formPA agents),
 split, simp at *, split, exact h3, exact ih1,
 exact imp_and_imp ih2
 end
 
-lemma exercise1 {AX Γ : ctx} {φ : form} {L : list form} :
-  max_ax_consist AX Γ → (∀ ψ ∈ L, ψ ∈ Γ) → prfK AX (fin_conj L ⊃ φ) → φ ∈ Γ :=
+lemma exercise1 {AX Γ : ctx agents} {φ : formPA agents} {L : list (formPA agents)} :
+  max_ax_consist AX Γ → (∀ ψ ∈ L, ψ ∈ Γ) → prfPA AX (fin_conj L ⊃ φ) → φ ∈ Γ :=
 begin
 intros h1 h2 h3, 
 by_contradiction h4, 
@@ -428,107 +431,105 @@ specialize h1 L'' h7, apply h1,
 exact cut h8 h6
 end
 
-lemma max_dn (AX Γ : ctx) (h : max_ax_consist AX Γ) (φ : form) :
-  φ ∈ Γ ↔ (¬¬φ) ∈ Γ :=
+lemma max_dn (AX Γ : ctx agents) (h : max_ax_consist AX Γ) (φ : formPA agents) :
+  φ ∈ Γ ↔ (~~φ) ∈ Γ :=
 begin
 split, intro h1, 
-have h2 : (∀ ψ ∈ [φ], ψ ∈ Γ) → prfK AX (fin_conj [φ] ⊃ (¬¬φ)) → (¬¬φ) ∈ Γ, from exercise1 h,
+have h2 : (∀ ψ ∈ [φ], ψ ∈ Γ) → prfPA AX (fin_conj [φ] ⊃ (~~φ)) → (~~φ) ∈ Γ, from exercise1 h,
 simp at *, apply h2, exact h1,
 repeat {rw fin_conj},
 exact (cut (mp pl5 phi_and_true) dni), 
 intro h1,
-have h2 : (∀ ψ ∈ [¬¬φ], ψ ∈ Γ) → prfK AX (fin_conj [¬¬φ] ⊃ φ) → φ ∈ Γ, from exercise1 h,
+have h2 : (∀ ψ ∈ [~~φ], ψ ∈ Γ) → prfPA AX (fin_conj [~~φ] ⊃ φ) → φ ∈ Γ, from exercise1 h,
 simp at *, apply h2, exact h1,
 repeat {rw fin_conj},
 exact (cut (mp pl5 phi_and_true) dne), 
 end
 
-lemma max_boxdn (AX Γ : ctx) (h : max_ax_consist AX Γ) (φ : form) :
-  (¬□φ) ∈ Γ → (¬□(¬¬φ)) ∈ Γ :=
+lemma max_boxdn (AX Γ : ctx agents) (h : max_ax_consist AX Γ) (φ : formPA agents) (a : agents) :
+  (~K a φ) ∈ Γ → (~K a (~~φ)) ∈ Γ :=
 begin
 intro h1,
-have h2 : (∀ ψ ∈ [(¬□φ)], ψ ∈ Γ) → prfK AX (fin_conj [(¬□φ)] ⊃ (¬□(¬¬φ))) → (¬□(¬¬φ)) ∈ Γ, 
+have h2 : (∀ ψ ∈ [(~K a φ)], ψ ∈ Γ) → prfPA AX (fin_conj [(~ (K a) φ)] ⊃ (~K a (~~φ))) → (~K a (~~φ)) ∈ Γ, 
   from exercise1 h,
 simp at *, apply h2, exact h1, clear h2,
 repeat {rw fin_conj at *},
 exact (cut (mp pl5 phi_and_true) (mp pl5 box_dn)), 
 end
 
-lemma max_notiff (AX Γ : ctx) (h : max_ax_consist AX Γ) (φ : form) :
-  φ ∉ Γ ↔ (¬φ) ∈ Γ :=
+lemma max_notiff (AX Γ : ctx agents) (h : max_ax_consist AX Γ) (φ : formPA agents) :
+  φ ∉ Γ ↔ (~φ) ∈ Γ :=
 begin
 split, intro h1,
 have h2 : ax_consist AX Γ, from max_imp_ax h, 
-have h3 : ∀ φ : form, φ ∈ Γ ∨ (¬φ) ∈ Γ, from six_helper AX Γ h2 h,
+have h3 : ∀ φ : formPA agents, φ ∈ Γ ∨ (~φ) ∈ Γ, from six_helper AX Γ h2 h,
 specialize h3 φ, cases h3, exact absurd h3 h1, exact h3,
 intro h1,
 have h2 : ax_consist AX Γ, from max_imp_ax h, 
-have h3 : max_ax_consist AX Γ ↔ ∀ φ, (φ ∈ Γ ∨ (¬φ) ∈ Γ) ∧ ¬(φ ∈ Γ ∧ (¬φ) ∈ Γ), 
+have h3 : max_ax_consist AX Γ ↔ ∀ φ, (φ ∈ Γ ∨ (~φ) ∈ Γ) ∧ ¬(φ ∈ Γ ∧ (~φ) ∈ Γ), 
   from six AX Γ h2,
-cases h3, specialize h3_mp h (¬φ), simp at *,
+cases h3, specialize h3_mp h (~φ), simp at *,
 cases h3_mp with mp1 mp2, specialize mp2 h1,
-have h4 : φ ∈ Γ ↔ (¬¬φ) ∈ Γ, from max_dn AX Γ h φ,
+have h4 : φ ∈ Γ ↔ (~~φ) ∈ Γ, from max_dn AX Γ h φ,
 rw ←not_iff_not at h4, cases h4, apply h4_mpr, exact mp2
 end
 
-lemma max_imp_1 {AX Γ : ctx} {φ ψ : form} : 
+lemma max_imp_1 {AX Γ : ctx agents} {φ ψ : formPA agents} : 
   max_ax_consist AX Γ → (φ ∈ Γ → ψ ∈ Γ) → (φ ⊃ ψ) ∈ Γ :=
 begin
 intros h1 h2, rw imp_iff_not_or at h2,
 cases h2,
-have h3 : (∀ χ ∈ [¬φ], χ ∈ Γ) → prfK AX (fin_conj [¬φ] ⊃ (φ ⊃ ψ)) → (φ ⊃ ψ) ∈ Γ, from exercise1 h1,
+have h3 : (∀ χ ∈ [~φ], χ ∈ Γ) → prfPA AX (fin_conj [~φ] ⊃ (φ ⊃ ψ)) → (φ ⊃ ψ) ∈ Γ, from exercise1 h1,
 simp at *, apply h3, 
 exact (max_notiff AX Γ h1 φ).mp h2,
 repeat {rw fin_conj at *},
-simp at *,
-have h4 : prfK AX ((¬φ) ⊃ (φ ⊃ ψ)), from and_right_imp.mp exfalso,
-simp at *,
+have h4 : prfPA AX ((~φ) ⊃ (φ ⊃ ψ)), from and_right_imp.mp exfalso,
 exact cut (mp pl5 phi_and_true) h4,
-have h3 : (∀ χ ∈ [ψ], χ ∈ Γ) → prfK AX (fin_conj [ψ] ⊃ (φ ⊃ ψ)) → (φ ⊃ ψ) ∈ Γ, from exercise1 h1,
+have h3 : (∀ χ ∈ [ψ], χ ∈ Γ) → prfPA AX (fin_conj [ψ] ⊃ (φ ⊃ ψ)) → (φ ⊃ ψ) ∈ Γ, from exercise1 h1,
 simp at *, 
 apply h3, exact h2, exact (cut (mp pl5 phi_and_true) pl1),
 end
 
-lemma max_imp_2 {AX Γ : ctx} {φ ψ : form} : 
+lemma max_imp_2 {AX Γ : ctx agents} {φ ψ : formPA agents} : 
   max_ax_consist AX Γ → (φ ⊃ ψ) ∈ Γ → φ ∈ Γ → ψ ∈ Γ :=
 begin
 intros h1 h2 h3,
-have h4 : (∀ χ ∈ [φ, (φ ⊃ ψ)], χ ∈ Γ) → prfK AX (fin_conj [φ, (φ ⊃ ψ)] ⊃ ψ) → ψ ∈ Γ, from exercise1 h1,
+have h4 : (∀ χ ∈ [φ, (φ ⊃ ψ)], χ ∈ Γ) → prfPA AX (fin_conj [φ, (φ ⊃ ψ)] ⊃ ψ) → ψ ∈ Γ, from exercise1 h1,
 simp at *, apply h4, intros χ h5, cases h5, subst h5, exact h3, subst h5, exact h2,
-repeat {rw fin_conj}, simp at *,
+repeat {rw fin_conj},
 exact and_right_imp.mpr (mp pl5 phi_and_true)
 end
 
-lemma max_conj_1 {AX Γ : ctx} {φ ψ : form} : 
+lemma max_conj_1 {AX Γ : ctx agents} {φ ψ : formPA agents} : 
   max_ax_consist AX Γ → (φ ∈ Γ ∧ ψ ∈ Γ) → (φ & ψ) ∈ Γ :=
 begin
 intros h1 h2, cases h2,
-have h3 : (∀ χ ∈ [φ], χ ∈ Γ) → prfK AX (fin_conj [φ] ⊃ (ψ ⊃ (φ & ψ))) → (ψ ⊃ (φ & ψ)) ∈ Γ, 
+have h3 : (∀ χ ∈ [φ], χ ∈ Γ) → prfPA AX (fin_conj [φ] ⊃ (ψ ⊃ (φ & ψ))) → (ψ ⊃ (φ & ψ)) ∈ Γ, 
   from exercise1 h1,
 simp at *, specialize h3 h2_left,
 repeat {rw fin_conj at *},
-have h5 : prfK AX ((φ&¬⊥)⊃(ψ⊃φ&ψ)),
+have h5 : prfPA AX ((φ&~⊥)⊃(ψ⊃φ&ψ)),
 exact (cut (mp pl5 phi_and_true) pl4), 
 specialize h3 h5,
 have h6 : (ψ ⊃ (φ & ψ)) ∈ Γ → ψ ∈ Γ → (φ & ψ) ∈ Γ, from max_imp_2 h1,
 apply h6, exact h3, exact h2_right
 end
 
-lemma max_conj_2 {AX Γ : ctx} {φ ψ : form} : 
+lemma max_conj_2 {AX Γ : ctx agents} {φ ψ : formPA agents} : 
   max_ax_consist AX Γ → (φ & ψ) ∈ Γ → φ ∈ Γ :=
 begin
 intros h1 h2,
-have h3 : (∀ χ ∈ [(φ & ψ)], χ ∈ Γ) → prfK AX (fin_conj [(φ & ψ)] ⊃ φ) → φ ∈ Γ, 
+have h3 : (∀ χ ∈ [(φ & ψ)], χ ∈ Γ) → prfPA AX (fin_conj [(φ & ψ)] ⊃ φ) → φ ∈ Γ, 
   from exercise1 h1,
 simp at *, apply h3, exact h2, repeat {rw fin_conj},
 exact (cut (mp pl5 phi_and_true) pl5)
 end
 
-lemma max_conj_3 {AX Γ : ctx} {φ ψ : form} : 
+lemma max_conj_3 {AX Γ : ctx agents} {φ ψ : formPA agents} : 
   max_ax_consist AX Γ → (φ & ψ) ∈ Γ → ψ ∈ Γ :=
 begin
 intros h1 h2,
-have h3 : (∀ χ ∈ [(φ & ψ)], χ ∈ Γ) → prfK AX (fin_conj [(φ & ψ)] ⊃ ψ) → ψ ∈ Γ, 
+have h3 : (∀ χ ∈ [(φ & ψ)], χ ∈ Γ) → prfPA AX (fin_conj [(φ & ψ)] ⊃ ψ) → ψ ∈ Γ, 
   from exercise1 h1,
 simp at *, apply h3, exact h2, repeat {rw fin_conj},
 exact (cut (mp pl5 phi_and_true) pl6)
@@ -536,7 +537,7 @@ end
 
 -- Γ is maximally AX-consistent iff it is AX-consistent and for 
 -- every AX-consistent set Γ', if Γ ⊆ Γ', then Γ = Γ'
-lemma max_equiv (AX Γ : ctx) : max_ax_consist AX Γ ↔ ax_consist AX Γ ∧ 
+lemma max_equiv (AX Γ : ctx agents) : max_ax_consist AX Γ ↔ ax_consist AX Γ ∧ 
   ∀ Γ', ax_consist AX Γ' → Γ ⊆ Γ' → Γ = Γ' :=
 begin
 split, 
@@ -560,7 +561,7 @@ open zorn
 -- by induction on L.
 -- S := collection of max cons sets
 -- m := Γ'
-lemma lindenhelper (c : set ctx) (h : c.nonempty) (h1 : chain (⊆) c) (L : list form) :
+lemma lindenhelper (c : set (ctx agents)) (h : c.nonempty) (h1 : chain (⊆) c) (L : list (formPA agents)) :
 (∀ φ ∈ L, φ ∈ ⋃₀(c)) → ∃ m ∈ c, (∀ ψ ∈ L, ψ ∈ m) :=
 begin
 -- have H : c = ∅ ∨ c ≠ ∅, from dec_em (c = ∅),
@@ -580,7 +581,7 @@ specialize h2 L_hd,
 simp at h2,
 cases h2 with m' h2,
 cases h2 with h2 h4,
-existsi (m' ∪ m : ctx), 
+existsi (m' ∪ m : ctx agents), 
 have H : m' ∪ m ∈ c, 
 sorry,
 existsi (H : m' ∪ m ∈ c),
@@ -590,7 +591,7 @@ specialize ih ψ h5, exact set.mem_union_right m' ih
 end
 
 
-lemma lindenbaum (AX Γ : ctx) (hax : ax_consist AX Γ) : 
+lemma lindenbaum (AX Γ : ctx agents) (hax : ax_consist AX Γ) : 
   ∃ Γ', max_ax_consist AX Γ' ∧ Γ ⊆ Γ' :=
 begin
 let P := { Γ'' | Γ'' ⊇ Γ ∧ ax_consist AX Γ''},
@@ -620,7 +621,7 @@ end
 
 
 -- Corollary 8
-lemma max_ax_exists (AX : ctx) (hax : sem_cons AX) : ∃ Γ : ctx, max_ax_consist AX Γ :=
+lemma max_ax_exists (AX : ctx agents) (hax : sem_cons AX) : ∃ Γ : ctx agents, max_ax_consist AX Γ :=
 begin
 have h1 : ax_consist AX ∅,
 {rw ax_consist, intro L, intro h2, rw fin_ax_consist, 
@@ -628,5 +629,5 @@ have h3 := listempty h2, have this : ∅ = ∅, refl,
 specialize h3 this, subst h3, by_contradiction h4, 
 have h5 := mp dne, apply nprfalse AX hax, exact h5 h4},
 have h2 : ∃ Γ, max_ax_consist AX Γ ∧ ∅ ⊆ Γ, from lindenbaum AX ∅ h1, 
-cases h2 with Γ h2, cases h2 with h2 h3, existsi (Γ : ctx), apply h2
+cases h2 with Γ h2, cases h2 with h2 h3, existsi (Γ : ctx agents), apply h2
 end
