src/del/semantics/semanticsDEL.lean
@@ -5,7 +5,7 @@ import del.languageDEL del.syntax.syntaxDEL data.set.basic
 variable {agents : Type}
 open formPA 
 local attribute [instance] classical.prop_decidable
--- hi
+
 
 ---------------------- Semantics ----------------------
 
@@ -46,35 +46,35 @@ def f_valid (φ : formPA agents) (f : frame agents) :=
 def F_valid (φ : formPA agents) (F : set (frame agents)) := 
   ∀ f ∈ F, ∀ v x, forces f v x φ
 
--- φ is universally valid (valid in all frames)
-def u_valid (φ : formPA agents) := 
-  ∀ f v x, forces f v x φ
+-- -- φ is universally valid (valid in all frames)
+-- def u_valid (φ : formPA agents) := 
+--   ∀ f v x, forces f v x φ
 
 -- A context is true at a world in a model if each 
 -- formula of the context is true at that world in that model
 def forces_ctx (f : frame agents) (v : nat → f.states → Prop) 
-  (x : f.states) (Γ : ctx agents) := ∀ φ, (φ ∈ Γ → forces f v x φ)
+  (Γ : ctx agents) := ∀ φ, ∀ x, φ ∈ Γ → forces f v x φ
 
--- I'm not sure which definition to use...
-def sem_csq2 (Γ : ctx agents) (φ : formPA agents) :=
-  ∀ f v x, (∀ y, forces_ctx f v y Γ) → forces f v x φ
+-- Local semantic consequence
+def local_sem_csq (Γ : ctx agents) (φ : formPA agents) :=
+  ∀ f v x, forces_ctx f v Γ → forces f v x φ
+
+-- Global semantic consequence
+def global_sem_csq (Γ : ctx agents) (φ : formPA agents) :=
+  ∀ f v x, forces_ctx f v Γ → forces f v x φ
 
 
-section
-open classical
 open set
 variables (f : frame agents) {α : Type} (a : agents) (r : α → α → Prop)
 
 def euclidean := ∀ ⦃x y z⦄, r x y → r x z → r y z 
 
-def ref_class : set (frame agents) := { f : frame agents | ∀ a : agents, reflexive (f.rel a) }
-def symm_class : set (frame agents) := { f : frame agents | ∀ a : agents, symmetric (f.rel a) }
-def trans_class : set (frame agents ) := { f : frame agents | ∀ a : agents, transitive (f.rel a) }
+--def ref_class : set (frame agents) := { f : frame agents | ∀ a : agents, reflexive (f.rel a) }
+--def symm_class : set (frame agents) := { f : frame agents | ∀ a : agents, symmetric (f.rel a) }
+--def trans_class : set (frame agents ) := { f : frame agents | ∀ a : agents, transitive (f.rel a) }
 def euclid_class : set (frame agents ) := { f : frame agents | ∀ a : agents, euclidean (f.rel a) }
-def ref_trans_class : set (frame agents) := ref_class ∩ trans_class
+--def ref_trans_class : set (frame agents) := ref_class ∩ trans_class
 def equiv_class : set (frame agents) := { f : frame agents | ∀ a : agents, equivalence (f.rel a) }
-
-end
 
 
 lemma not_forces_imp (f : frame agents) : ∀ v x φ, 
@@ -85,9 +85,30 @@ intros v x φ, split,
 {intros h1 h2, specialize h1 h2, exact h1}
 end
 
+lemma forces_exists {a : agents} {f : frame agents} {v : nat → f.states → Prop} {x : f.states} {φ : formPA agents} :
+  forces f v x (~K a ~φ) ↔ ∃ y : f.states, (f.rel a x y ∧ forces f v y φ) :=
+begin
+split,
+intro h1,
+rw forces at h1, rw forces at h1,
+have h2 := not_or_of_imp h1,
+clear h1, cases h2, push_neg at h2,
+cases h2 with y h2, cases h2 with h2 h3,
+existsi (y : f.states), split, exact h2,
+have h4 := (not_forces_imp f v y (~φ)).mp h3,
+repeat {rw forces at h4}, repeat {rw imp_false at h4},
+rw not_not at h4, exact h4,
+rw forces at h2, exact false.elim h2,
+intro h1, cases h1 with y h1,
+cases h1 with h1 h2,
+rw forces,
+intro h3,
+rw forces at h3, specialize h3 y h1,
+rw ←not_forces_imp at h3, 
+exact absurd h2 h3
+end
 
-
-lemma forces_exists (φ ψ : formPA agents) (f : frame agents) (v : nat → f.states → Prop) (x : f.states) : 
+lemma forces_update_dual (φ ψ : formPA agents) (f : frame agents) (v : nat → f.states → Prop) (x : f.states) : 
 forces f v x ~(U φ (~ψ)) ↔ ∃ h : forces f v x φ, 
       forces (f.restrict (λ y, forces f v y φ) x h) (λ n u, v n u.val) ⟨x, h⟩ ψ :=
 begin
